supporting shl

coq/examples/test_15.c
@@ -1,0 +1,21 @@
+#include <stdlib.h>
+#include <stdbool.h>
+#include <stdint.h>
+#include <assert.h>
+
+#include <klee/klee.h>
+
+void f1(int x) {
+    int y = x << 2;
+}
+
+void f2() {
+    int x = klee_make_symbolic_int32();
+    int y = x << 7;
+}
+
+int main() {
+    f1(100);
+    f2();
+    return 0;
+}
