coq/ExecutionTreeOpt.v
@@ -249,6 +249,37 @@ Proof.
     ).
   }
   {
+    destruct (sym_eval_exp ls1 gs1 (Some (TYPE_I w)) e1) as [se1' | ] eqn:E1; try discriminate Heval.
+    destruct (sym_eval_exp ls1 gs1 (Some (TYPE_I w)) (EXP_Integer n)) as [se2' | ] eqn:E2; try discriminate Heval.
+    apply IHe1 with (ot := Some (TYPE_I w)) (se1 := se1') in H4; try assumption.
+    destruct H4 as [se1'' [H4_1 H4_2]].
+    assert(L : is_supported_exp (EXP_Integer n)).
+    { apply IS_EXP_Integer. }
+    apply IHe2 with (ot := Some (TYPE_I w)) (se1 := se2') in L; try assumption.
+    destruct L as [se2'' [L_1 L_2]].
+    simpl in L_1.
+    simpl.
+    rewrite H4_1, L_1.
+    destruct se1 as [sort1 ast1].
+    destruct se1' as [sort1' ast1'].
+    destruct se2' as [sort2' ast2'].
+    destruct se1'' as [sort1'' ast1''].
+    destruct se2'' as [sort2'' ast2''].
+    assert(L1 : sort1' = sort1'').
+    { apply sort_injection in H4_2. assumption. }
+    assert(L2 : sort2' = sort2'').
+    { apply sort_injection in L_2. assumption. }
+    subst.
+    destruct sort1'', sort2''; try discriminate Heval;
+    (
+      inversion H3; subst;
+      inversion Heval; subst;
+      eexists;
+      split; try reflexivity;
+      apply equiv_smt_expr_binop; assumption
+    ).
+  }
+  {
     destruct (sym_eval_exp ls1 gs1 (Some t) e1) as [se1' | ] eqn:E1; try discriminate Heval.
     destruct (sym_eval_exp ls1 gs1 (Some t) e2) as [se2' | ] eqn:E2; try discriminate Heval.
     apply IHe1 with (ot := Some t) (se1 := se1') in H1; try assumption.
